SATsolver/Experiment/DPLL/Theorem.lean
@@ -1,7 +1,7 @@
 import SATsolver.Experiment.DPLL.impl
 
 theorem internal_final_state{f: Formula}{v : Variables}{vz : v ≠ 0}{wf : f.wf ∧ v.wf f}{b : Bool}{t t' : Trail}{twf : t.wf ∧ ∀ n ∈ t.names, n ∈ f.names}{com : Completenes.inv t f}:
-  internal t f v vz wf twf com = (b, t') → t' ⊨ f ∨ b = false := by
+  internal t f v vz wf twf com = (b, t') → (b = true ∧ t' ⊨ f) ∨ b = false := by
   unfold internal
   split
   case isTrue hsat =>
@@ -50,13 +50,74 @@ decreasing_by
   exact distance_bc this
 
 theorem DPLL.final_state{f : Formula}{v : Variables}{wf : f.wf ∧ v.wf f}{b : Bool}{t : Trail}:
-DPLL f  v wf = (b, t) → t ⊨ f ∨ b = false := by
+DPLL f  v wf = (b, t) → (b = true ∧ t ⊨ f) ∨ b = false := by
   simp[DPLL]
   cases f
   case nil => simp[Satisfies.sat]
   case cons c cs =>
     simp
     exact internal_final_state
+
+
+theorem internal_wf{f: Formula}{v : Variables}{vz : v ≠ 0}{wf : f.wf ∧ v.wf f}{b : Bool}{t t' : Trail}{twf : t.wf ∧ ∀ n ∈ t.names, n ∈ f.names}{com : Completenes.inv t f}:
+  internal t f v vz wf twf com = (b, t') → t'.wf := by
+  unfold internal
+  split
+  case isTrue hsat =>
+    simp at hsat ⊢
+    intro bh heq
+    simp[←heq, twf.1]
+  case isFalse hsat =>
+    split
+    case isTrue hcon =>
+      split
+      case isTrue exDec =>
+        intro h
+        exact internal_wf h
+      case isFalse exDec =>
+        simp
+        intro bh th
+        simp[←th, twf.1]
+    case isFalse hcon =>
+      simp
+      split
+      case isTrue hunit =>
+        intro h
+        exact internal_wf h
+      case isFalse hunit =>
+        intro h
+        exact internal_wf h
+termination_by distance t v vz
+decreasing_by
+  have : t.length < v := by
+    rename ¬decide (t⊨f) = true => sat
+    rename ¬decide (t⊭f) = true => con
+    simp at sat con
+    have := Trail.ud_vars twf.1 wf.1 wf.2 twf.2 (Formula.nSatCon_ud sat con)
+    simp[Trail.names] at this
+    exact this
+  exact distance_dec this
+  have : t.length < v := by
+    rename ¬decide (t⊨f) = true => sat
+    rename ¬decide (t⊭f) = true => con
+    simp at sat con
+    have := Trail.ud_vars twf.1 wf.1 wf.2 twf.2 (Formula.nSatCon_ud sat con)
+    simp[Trail.names] at this
+    exact this
+  exact distance_prop this
+  have : t.length ≤ v := Trail.mem_vwf twf.1 twf.2 wf.2
+  exact distance_bc this
+
+
+theorem DPLL.wf{f : Formula}{v : Variables}{wf : f.wf ∧ v.wf f}{b : Bool}{t : Trail}:
+DPLL f  v wf = (b, t) → t.wf := by
+  simp[DPLL]
+  cases f
+  case nil => simp; intro bh heq; simp[heq, Trail.wf, Trail.names]
+  case cons c cs =>
+    simp
+    exact internal_wf
+
 
 theorem internal_all_deduced_if_con{f: Formula}{v : Variables}{vz : v ≠ 0}{wf : f.wf ∧ v.wf f}{b : Bool}{t t' : Trail}{twf : t.wf ∧ ∀ n ∈ t.names, n ∈ f.names}{com : Completenes.inv t f}:
   internal t f v vz wf twf com = (b, t') → b = false → (t' ⊭ f ∧  ∀ a ∈ t', a.deducedP) := by
@@ -192,64 +253,35 @@ theorem DPLL.soundness {f : Formula}{v : Variables}{wf : f.wf ∧ v.wf f}{b : Bo
   simp[bh] at this
   exists t
 
-theorem DPLL.final_false{f: Formula}{v : Variables}{vz : v ≠ 0}{wf : f.wf ∧ v.wf f}{t t' : Trail}{twf : t.wf ∧ ∀ n ∈ t.names, n ∈ f.names}:
+theorem DPLL.final_false {b : Bool}{f: Formula}{v : Variables}{wf : f.wf ∧ v.wf f}{t : Trail}{twf : t.wf}:
   DPLL f v wf = (b, t) → b = false → ¬ (∃ (t : Trail), t.wf ∧ t ⊨ f) := by
   intro heq bfalse
   have state := DPLL.all_deduced_if_con heq bfalse
   have com := DPLL.com_preserved heq
-  have := Completenes.inv_completeness twf.1 com state.2
+  have := Completenes.inv_completeness twf com state.2
   simp at this ⊢
   intro x xwf
   have nohead := Completenes.from_con state.1
   simp at nohead
-
-
-  intro h
-  unfold internal at h
-  split at h
-  case isTrue hsat => simp at h
-  case isFalse hsat =>
-    split at h
-    case isTrue hcon =>
-      simp at h
-      split at h
-      case isTrue hexi =>
-        exact internal_final_false h
-      case isFalse hexi =>
-        simp at hexi
-
+  exact this nohead x xwf
 
 
 theorem DPLL.completeness {f : Formula}{v : Variables}{wf : f.wf ∧ v.wf f}:
-  (∃ (t : Trail), t ⊨ f) → ∃ (t : Trail), DPLL f v wf = (true, t) := by
+  (∃ (t : Trail), t.wf ∧ t ⊨ f) → ∃ (t : Trail), DPLL f v wf = (true, t) := by
   intro h
-  obtain ⟨ t, tsat ⟩ := h
-  simp[DPLL]
-  split
-  case h_1 => simp
-  case h_2 f wf hd tl wf' =>
-    unfold internal
-    split
-    case isTrue hsat => simp
-    case isFalse hsat =>
-      split
-      case isTrue hcon =>
-        simp[Conflict.con, Trail.lits] at hcon
-        simp[Formula.wf, Clause.wf] at wf'
-        have := wf'.1.1.1.1
-        obtain ⟨ l, ls, lmem ⟩ := List.ne_nil_iff_exists_cons.mp this
-        cases hcon
-        case inl hcon =>
-          simp[lmem] at hcon
-          have := hcon l
-          simp at this
-        case inr hcon =>
-          obtain ⟨ c, cmem, call ⟩ := hcon
-          have := (wf'.1.2 c cmem).1.1
-          obtain ⟨ l, ls, lmem ⟩ := List.ne_nil_iff_exists_cons.mp this
-          simp[lmem] at call
-          have := call l
-          simp at this
-      case isFalse hcon =>
-        simp
-        split
+  obtain ⟨ t, twf, tsat ⟩ := h
+  let dpll : (Bool ×  Trail) := DPLL f v wf
+  let b := dpll.1
+  let t' := dpll.2
+  have dplleq : DPLL f v wf = (b, t') := by simp[dpll, b ,t']
+  have := DPLL.final_state dplleq
+  cases this
+  case inl lh =>
+    exists t'
+    rw[dplleq, lh.1]
+  case inr rh =>
+    have := DPLL.wf dplleq
+    have := DPLL.final_false (twf := this) dplleq rh
+    simp at this
+    have := this t twf
+    contradiction
