SATsolver/Experiment/Relations/Satisfies.lean
@@ -48,10 +48,80 @@ def Formula.sat_iff_all_csSat {f : Formula}{t : Trail} :
 theorem sat_remapp_sat{t : Trail}{f : Formula}{a : ALit} :
   t.wf → a ∈ t → (t⊨ f  ↔ (t.remove a.name ++ [a]) ⊨ f) := by
   intro twf amem
-  have : (t.remove a.name ++ [a]).wf := Trail.wf_remapp twf amem
-  have := Trail.remove_eq twf amem amem
-  simp[Satisfies.sat] at *
-  intro c cmem
-  obtain ⟨ l, lc, lt ⟩ := sat c cmem
-  exists l
-  simp[lc, Trail.lits_append, Trail.remove]
+  have remwf: (t.remove a.name ++ [a]).wf := Trail.wf_remapp twf amem
+  simp[Satisfies.sat]
+  constructor
+  case mp =>
+    intro call c cmem
+    obtain ⟨ l, lc, lt ⟩ := call c cmem
+    exists l
+    simp[lc]
+    obtain ⟨ b, bmem, bheq ⟩ := Trail.mem_lits_exists_mem lt
+    cases Trail.remove_eq twf bmem amem
+    case inl lh =>
+      have := Trail.mem_mem_lits lh
+      rw[Trail.lits_append]
+      simp[←bheq, this]
+    case inr rh =>
+      simp[←bheq, rh, Trail.lits]
+  case mpr =>
+    intro call c cmem
+    obtain ⟨ l, lc, lt ⟩ := call c cmem
+    exists l
+    simp[lc]
+    obtain ⟨ b, bmem, bheq ⟩ := Trail.mem_lits_exists_mem lt
+    simp[Trail.remove] at bmem
+    cases bmem
+    case inl lh =>
+      have := Trail.mem_mem_lits lh.1
+      simp[←bheq, this]
+    case inr rh =>
+      have := Trail.mem_mem_lits amem
+      simp[←bheq, rh, this]
+
+
+theorem appsat_remapp_sat{hd tl : Trail}{f : Formula}{a : ALit} :
+  (hd++tl).wf → a ∈ hd → (hd++tl⊨ f ↔ (hd.remove a.name ++ [a]++tl) ⊨ f) := by
+  intro twf amem
+  constructor
+  case mp =>
+    intro h
+    simp[Satisfies.sat] at h ⊢
+    intro c cmem
+    obtain ⟨ l, lc, lt ⟩ := h c cmem
+    exists l
+    simp[lc, Trail.lits] at lt ⊢
+    cases lt
+    case inl lh =>
+      obtain ⟨ b, bmem, bheq ⟩ := lh
+      by_cases heq : a = b
+      case pos => simp[heq, bheq]
+      case neg =>
+        left
+        exists b
+        have := Trail.uniques (Trail.wf_append twf).1 heq amem bmem
+        simp[Trail.remove, bmem, bheq]
+        intro contra
+        simp[contra] at this
+    case inr rh => right; right; exact rh
+  case mpr =>
+    intro h
+    simp[Satisfies.sat] at h ⊢
+    intro c cmem
+    obtain ⟨ l, lc, lt ⟩ := h c cmem
+    exists l
+    simp[lc, Trail.lits] at lt ⊢
+    cases lt
+    case inl lh =>
+      obtain ⟨ b, bmem, bheq ⟩ := lh
+      have := Trail.mem_remove_mem  bmem
+      left
+      exists b
+    case inr rh =>
+      cases rh
+      case inl lh =>
+        left
+        exists a
+        simp[amem, lh]
+      case inr rh =>
+        simp[rh]
